src/Language/PlutusIR/Semantics/Dynamic.v
@@ -1,4 +1,11 @@
+(** ** Definition of big-step semantics *)
 Require Export PlutusCert.Language.PlutusIR.Semantics.Dynamic.Bigstep.
 Require Export PlutusCert.Language.PlutusIR.Semantics.Dynamic.BuiltinMeanings.
 Require Export PlutusCert.Language.PlutusIR.Semantics.Dynamic.Substitution.
 Require Export PlutusCert.Language.PlutusIR.Semantics.Dynamic.Values.
+
+(** ** Theorems and lemmas about the big-step semantics *)
+Require Export PlutusCert.Language.PlutusIR.Semantics.Dynamic.Bigstep.Congruence.
+Require Export PlutusCert.Language.PlutusIR.Semantics.Dynamic.Bigstep.Deterministic.
+Require Export PlutusCert.Language.PlutusIR.Semantics.Dynamic.Bigstep.EvalToValue.
+Require Export PlutusCert.Language.PlutusIR.Semantics.Dynamic.Bigstep.EvalValue.
