src/Language/PlutusIR/Semantics/Dynamic/Bigstep/Congruence.v
@@ -1,0 +1,41 @@
+Require Import PlutusCert.Language.PlutusIR.
+Import NamedTerm.
+Require Import PlutusCert.Language.PlutusIR.Semantics.Dynamic.Bigstep.
+Require Import PlutusCert.Language.PlutusIR.Semantics.Dynamic.Bigstep.EvalToValue.
+Require Import PlutusCert.Language.PlutusIR.Semantics.Dynamic.Bigstep.EvalValue.
+Require Import PlutusCert.Language.PlutusIR.Semantics.Dynamic.Bigstep.Deterministic.
+
+Lemma eval_congr_Apply1 : forall t1 t2 v1 v0,
+    Apply t1 t2 ==> v0 ->
+    t1 ==> v1 ->
+    Apply v1 t2 ==> v0.
+Proof.
+  intros.
+  inversion H; subst.
+  - assert (v1 = LamAbs x T t4) by (eapply eval__deterministic; eauto).
+    subst.
+    apply E_Apply with x T t4 t0' v2.
+    + apply E_LamAbs.
+    + assumption.
+    + assumption.
+    + assumption.
+  - assert (v1 = v2) by (eapply eval__deterministic; eauto).
+    subst.
+    apply E_ApplyBuiltin1.
+    + apply eval_value.
+      apply V_Builtin.
+      assumption.
+    + assumption.
+    + assumption.
+    + assumption.
+  - assert (v1 = v2) by (eapply eval__deterministic; eauto).
+    subst.
+    eapply E_ApplyBuiltin2.
+    + apply eval_value.
+      apply V_Builtin.
+      assumption.
+    + assumption.
+    + apply H5.
+    + assumption.
+    + assumption.
+Qed.
