src/Language/PlutusIR/Semantics/SemanticEquivalence/Def.v
@@ -10,8 +10,8 @@ Notation beta_reduce := (beta_reduce tyname binderTyname substituteT).
    type substitution and beta reduction. However, Coq can then not
    guess the decreasing argument of fix anymore. *)
 Fixpoint R (T : Ty) (t1 t2 : Term) : Prop :=
-  empty |-+ t1 : T /\
-  empty |-+ t2 : T /\
+  emptyContext |-+ t1 : T /\
+  emptyContext |-+ t2 : T /\
   exists v1 v2,
     t1 ==> v1 /\
     t2 ==> v2 /\
@@ -43,17 +43,17 @@ Fixpoint R (T : Ty) (t1 t2 : Term) : Prop :=
 
 Lemma R_typable_empty : forall T t1 t2,
     R T t1 t2 ->
-    empty |-+ t1 : T /\ empty |-+ t2 : T.
+    emptyContext |-+ t1 : T /\ emptyContext |-+ t2 : T.
 Proof. intros. destruct T; destruct H as [Ht1 [Ht2 _]]; auto. Qed.
 
 Lemma R_typable_empty_1 : forall T t1 t2,
     R T t1 t2 ->
-    empty |-+ t1 : T.
+    emptyContext |-+ t1 : T.
 Proof. intros. destruct (R_typable_empty _ _ _ H). assumption. Qed.
 
 Lemma R_typable_empty_2 : forall T t1 t2,
     R T t1 t2 ->
-    empty |-+ t2 : T.
+    emptyContext |-+ t2 : T.
 Proof. intros. destruct (R_typable_empty _ _ _ H). assumption. Qed.
 
 Lemma R_evaluable : forall T t1 t2,
@@ -89,8 +89,17 @@ Lemma R_functional_extensionality : forall T1 T2 t1 t2,
       R T2 (Apply v1 s1) (Apply v2 s2)).
 Proof. intros. destruct H as [_ [_ [v1 [v2 [Hev1 [Hev2 Hfe]]]]]]. eauto. Qed.
 
-
-
+Lemma R_falsity : forall t1 t2,
+  (forall a, ~(R (Ty_Var a) t1 t2)) /\
+  (forall bX K T, ~(R (Ty_Lam bX K T) t1 t2)) /\
+  (forall T1 T2, ~(R (Ty_App T1 T2) t1 t2)).
+Proof. 
+  split.
+  - intros. intro Hcon. destruct Hcon as [_ [_ [_ [_ [_ [_ Hfalse]]]]]]. destruct Hfalse.
+  - split.
+    + intros. intro Hcon. edestruct Hcon as [_ [_ [_ [_ [_ [_ Hfalse]]]]]]. destruct Hfalse.
+    + intros. intro Hcon. edestruct Hcon as [_ [_ [_ [_ [_ [_ Hfalse]]]]]]. destruct Hfalse.
+Qed.
 
 (* TODO: Possible fixes for R require a proof of well-founded recursion. I've tried out some things
    below, but I have not founda solution yet. *)
@@ -109,8 +118,8 @@ Fixpoint countBindingLocations (T : Ty) : nat :=
   end.
 
 Program Fixpoint R'' (T : Ty) (t1 t2 : Term) {measure (countBindingLocations T)} : Prop :=
-  empty |-+ t1 : T /\
-  empty |-+ t2 : T /\
+  emptyContext |-+ t1 : T /\
+  emptyContext |-+ t2 : T /\
   exists v1 v2,
     t1 ==> v1 /\
     t2 ==> v2 /\
@@ -119,7 +128,7 @@ Program Fixpoint R'' (T : Ty) (t1 t2 : Term) {measure (countBindingLocations T)}
         forall t0 T',
           v1 = TyAbs X K t0 ->
           v2 = TyAbs X K t0 ->
-          empty |-* T' : K ->
+          emptyContext |-* T' : K ->
           R'' (beta_reduce (substituteT X T' T0)) (TyInst v1 T') (TyInst v2 T')
     | Ty_Fun T1 T2 => 
         forall s1 s2,
@@ -129,7 +138,7 @@ Program Fixpoint R'' (T : Ty) (t1 t2 : Term) {measure (countBindingLocations T)}
         v1 = v2
     | Ty_IFix F T0 => 
         forall X K,
-          empty |-* T : K ->
+          emptyContext |-* T : K ->
           R'' (beta_reduce (unwrapIFix F X K T0)) (Unwrap v1) (Unwrap v2)
     |_ => False
     end.
@@ -145,8 +154,8 @@ Next Obligation. Admitted.
 (* WF by countBindingLocations and size? *)
 Equations R' (T : Ty) (t1 t2 : Term) : Prop by wf (countBindingLocations T) :=
   R' T t1 t2 =>
-    empty |-+ t1 : T /\
-    empty |-+ t2 : T /\
+    emptyContext |-+ t1 : T /\
+    emptyContext |-+ t2 : T /\
     exists v1 v2,
       t1 ==> v1 /\
       t2 ==> v2 /\
@@ -155,7 +164,7 @@ Equations R' (T : Ty) (t1 t2 : Term) : Prop by wf (countBindingLocations T) :=
           forall t0 T',
             v1 = TyAbs X K t0 ->
             v2 = TyAbs X K t0 ->
-            empty |-* T' : K ->
+            emptyContext |-* T' : K ->
             R' (beta_reduce (substituteT X T' T0)) (TyInst v1 T') (TyInst v2 T')
       | Ty_Fun T1 T2 => 
           forall s1 s2,
@@ -165,7 +174,7 @@ Equations R' (T : Ty) (t1 t2 : Term) : Prop by wf (countBindingLocations T) :=
           v1 = v2
       | Ty_IFix F T0 => 
           forall X K,
-            empty |-* T : K ->
+            emptyContext |-* T : K ->
             R' (beta_reduce (unwrapIFix F X K T0)) (Unwrap v1) (Unwrap v2)
       |_ => False
       end.
@@ -173,8 +182,8 @@ Equations R' (T : Ty) (t1 t2 : Term) : Prop by wf (countBindingLocations T) :=
 
 Fail Inductive R : Ty -> Term -> Term -> Prop :=
   | R_ : forall t1 t2 T,
-      (empty |-+ t1 : T /\
-      empty |-+ t2 : T /\
+      (emptyContext |-+ t1 : T /\
+      emptyContext |-+ t2 : T /\
       exists v1 v2,
         t1 ==> v1 /\
         t2 ==> v2 /\
@@ -186,8 +195,8 @@ with R2 : Ty -> Term -> Term -> Prop :=
       forall v1 v2 t0 T' S,
         v1 = TyAbs X K t0 ->
         v2 = TyAbs X K t0 ->
-        empty |-+ t0 : T0 ->
-        empty |-* T' : K ->
+        emptyContext |-+ t0 : T0 ->
+        emptyContext |-* T' : K ->
         substituteT X T' T0 =b S ->
         R S (TyInst v1 T') (TyInst v2 T') ->
         R2 (Ty_Forall X K T0) v1 v2
