src/Language/PlutusIR/Transform/LetNonRec/DSP.v
@@ -1,0 +1,925 @@
+Require Import PlutusCert.Language.PlutusIR.
+Import NamedTerm.
+Require Import PlutusCert.Language.PlutusIR.Transform.LetNonRec.
+Require Import PlutusCert.Language.PlutusIR.Transform.LetNonRec.SSP.
+Require Import PlutusCert.Language.PlutusIR.Semantics.Dynamic.
+Require Import PlutusCert.Language.PlutusIR.Semantics.Static.
+Require Import PlutusCert.Language.PlutusIR.Semantics.Static.Implementations.Named.
+Require Import PlutusCert.Language.PlutusIR.Semantics.TypeSafety.Preservation.
+Require Import PlutusCert.Language.PlutusIR.Semantics.TypeSafety.Progress.
+Require Import PlutusCert.Language.PlutusIR.Semantics.TypeSafety.SubstitutionPreservesTyping.
+Require Import PlutusCert.Language.PlutusIR.Semantics.SemanticEquivalence.Def.
+
+
+Require Import Coq.Lists.List.
+
+
+
+(** ** Context invariance *)
+
+Inductive appears_free_in : name -> Term -> Prop :=
+  | AFI_Let : forall x r bs t,
+      appears_free_in x t ->
+      appears_free_in x (Let r bs t)
+  | AFI_LetNonRec : forall x bs t,
+      appears_free_in_bindings_nonrec x bs ->
+      appears_free_in x (Let NonRec bs t)
+  | AFI_LetRec : forall x bs t,
+      ~(In x (term_vars_bound_by_bindings bs)) ->
+      appears_free_in_bindings_rec x bs ->
+      appears_free_in x (Let Rec bs t)
+  | AFI_Var : forall x,
+      appears_free_in x (Var x)
+  | AFI_TyAbs : forall x bX K t0,
+      appears_free_in x t0 ->
+      appears_free_in x (TyAbs bX K t0)
+  | AFI_LamAbs : forall x bx K t0,
+      appears_free_in x t0 ->
+      appears_free_in x (LamAbs bx K t0)
+  | AFI_Apply1 : forall x t1 t2,
+      appears_free_in x t1 ->
+      appears_free_in x (Apply t1 t2)
+  | AFI_Apply2 : forall x t1 t2,
+      appears_free_in x t2 ->
+      appears_free_in x (Apply t1 t2)
+  | AFI_TyInst : forall x t0 T,
+      appears_free_in x t0 ->
+      appears_free_in x (TyInst t0 T)
+  | AFI_IWrap : forall x F T t0,
+      appears_free_in x t0 ->
+      appears_free_in x (IWrap F T t0)
+  | AFI_Unwrap : forall x t0,
+      appears_free_in x t0 ->
+      appears_free_in x (Unwrap t0)
+
+with appears_free_in_bindings_nonrec : name -> list Binding -> Prop :=
+  | AFI_ConsB1_NonRec : forall x b bs,
+      appears_free_in_binding x b ->
+      appears_free_in_bindings_nonrec x (b :: bs)
+  | AFI_ConsB2_NonRec : forall x b bs,
+      ~(In x (term_vars_bound_by_binding b)) ->
+      appears_free_in_bindings_nonrec x bs ->
+      appears_free_in_bindings_nonrec x (b :: bs)
+
+with appears_free_in_bindings_rec : name -> list Binding -> Prop :=
+  | AFI_ConsB1_Rec : forall x b bs,
+      appears_free_in_binding x b ->
+      appears_free_in_bindings_rec x (b :: bs)
+  | AFI_ConsB2_Rec : forall x b bs,
+      appears_free_in_bindings_rec x bs ->
+      appears_free_in_bindings_rec x (b :: bs)
+
+with appears_free_in_binding : name -> Binding -> Prop :=
+  | AFI_TermBind : forall x s vd t0,
+      appears_free_in x t0 ->
+      appears_free_in_binding x (TermBind s vd t0)
+  .
+
+Definition closed (t : Term) :=
+  forall x, ~(appears_free_in x t).
+
+Lemma context_invariance : forall Gamma Gamma' t S,
+    Gamma |-+ t : S ->
+    (forall x, appears_free_in x t -> lookupT Gamma x = lookupT Gamma' x) ->
+    Gamma' |-+ t : S.
+Proof. Admitted.
+
+Lemma free_in_context : forall x t T Gamma,
+    appears_free_in x t ->
+    Gamma |-+ t : T ->
+    exists T', lookupT Gamma x = Datatypes.Some T'.
+Proof. Admitted.
+
+Corollary typable_empty__closed : forall t T,
+    emptyContext |-+ t : T ->
+    closed t.
+Proof.
+  intros. unfold closed. intros x H1.
+  destruct (free_in_context _ _ _ _ H1 H) as [T' C].
+  discriminate C.
+Qed.
+
+(** ** Multisubstitutions, multi-extensions, and instantiations *)
+
+Definition env := list (name * Term).
+
+Inductive msubst : env -> Term -> Term -> Prop :=
+  | msubst_nil : forall t,
+      msubst nil t t
+  | msubst_cons : forall x s ss t t' t'',
+      substitute x s t t' ->
+      msubst ss t' t'' ->
+      msubst ((x, s) :: ss) t t''
+  .
+
+Definition tass := list (name * Ty).
+
+Fixpoint mupdate (Gamma : Context) (xts : tass) :=
+  match xts with
+  | nil => Gamma
+  | ((x, v) :: xts') => extendT x v (mupdate Gamma xts')
+  end. 
+
+Fixpoint lookup {X:Type} (k : string) (l : list (name * X)) : option X :=
+  match l with
+  | nil => None
+  | (j,x) :: l' => if String.eqb j k then Datatypes.Some x else lookup k l'
+  end.
+
+Fixpoint drop {X:Type} (n:string) (nxs:list (string * X)) : list (string * X) :=
+  match nxs with
+  | nil => nil
+  | (n',x) :: nxs' => if String.eqb n' n then drop n nxs' else (n',x) :: (drop n nxs')
+  end.
+
+Inductive instantiation : tass -> env -> env -> Prop :=
+  | V_nil : 
+      instantiation nil nil nil
+  | V_cons : forall x T v1 v2 c e1 e2,
+      value v1 ->
+      value v2 ->
+      R T v1 v2 ->
+      instantiation c e1 e2 ->
+      instantiation ((x, T) :: c) ((x, v1) :: e1) ((x, v2) :: e2)
+  . 
+
+
+
+(** ** More substitution facts *)
+
+Definition P_Term (t : Term) :=
+  forall x,
+    ~(appears_free_in x t) ->
+    forall s t', 
+      substitute x s t t' ->
+      t' = t.
+
+Definition P_Binding (b : Binding) :=
+  forall x,
+    ~(appears_free_in_binding x b) ->
+    forall s b',
+      substitute_binding x s b b' ->
+      b' = b.
+
+Definition P_Bindings_NonRec (bs : list Binding) :=
+  Util.ForallT P_Binding bs ->
+  forall x,
+    ~(appears_free_in_bindings_nonrec x bs) ->
+    forall s bs',
+      substitute_bindings_nonrec x s bs bs' ->
+      bs' = bs.
+
+Lemma P_Bindings_NonRec__holds_definitionally : forall bs, P_Bindings_NonRec bs.
+Proof.
+  induction bs.
+  - unfold P_Bindings_NonRec. intros.
+    inversion H0. subst.
+    reflexivity.
+  - unfold P_Bindings_NonRec. intros.
+    inversion H0.
+    + subst.
+      f_equal.
+      apply Util.ForallT_hd in X.
+      unfold P_Binding in X.
+      apply X with x s.
+      * intros Hcon.
+        apply H.
+        apply AFI_ConsB1_NonRec.
+        assumption.
+      * assumption.
+    + subst.
+      f_equal.
+      * apply Util.ForallT_hd in X.
+        unfold P_Binding in X.
+        apply X with x s.
+        -- intros Hcon.
+           apply H.
+           apply AFI_ConsB1_NonRec.
+           assumption.
+        -- assumption.
+      * unfold P_Bindings_NonRec in IHbs.
+        apply IHbs with x s.
+        -- apply Util.ForallT_tl in X.
+           assumption.
+        -- intros Hcon.
+           apply H.
+           apply AFI_ConsB2_NonRec.
+           ++ assumption.
+           ++ assumption.
+        -- assumption.
+Qed.
+
+Definition P_Bindings_Rec (bs : list Binding) :=
+  Util.ForallT P_Binding bs ->
+  forall x,
+    ~(appears_free_in_bindings_rec x bs) ->
+    forall s bs',
+      substitute_bindings_rec x s bs bs' ->
+      bs' = bs.
+
+Lemma P_Bindings_Rec__holds_definitionally : forall bs, P_Bindings_Rec bs.
+Proof.
+  induction bs.
+  - unfold P_Bindings_Rec. intros.
+    inversion H0. subst.
+    reflexivity.
+  - unfold P_Bindings_Rec. intros.
+    inversion H0.
+    subst.
+    f_equal.
+    + apply Util.ForallT_hd in X.
+      unfold P_Binding in X.
+      apply X with x s.
+      * intros Hcon.
+        apply H.
+        apply AFI_ConsB1_Rec.
+        assumption.
+      * assumption.
+    + unfold P_Bindings_Rec in IHbs.
+      apply IHbs with x s.
+      * apply Util.ForallT_tl in X.
+        assumption.
+      * intros Hcon.
+        apply H.
+        apply AFI_ConsB2_Rec.
+        assumption.
+      * assumption.
+Qed.
+
+Lemma vacuous_substitution : forall t, P_Term t.
+Proof.
+  apply Term_rect' with (P := P_Term) (Q := P_Binding).
+  - (* Let *)
+    intros. unfold P_Term. intros.
+    inversion H1; subst.
+    + (* S_Let1 *)
+      f_equal.
+      assert (P_Bindings_NonRec bs) by apply P_Bindings_NonRec__holds_definitionally.
+      unfold P_Bindings_NonRec in H2.
+      apply H2 with x s.
+      * assumption.
+      * intros Hcon.
+        apply H0.
+        apply AFI_LetNonRec.
+        assumption.
+      * assumption.
+    + (* S_Let2 *)
+      f_equal.
+      * assert (P_Bindings_NonRec bs) by apply P_Bindings_NonRec__holds_definitionally.
+        unfold P_Bindings_NonRec in H2.
+        apply H2 with x s.
+        -- assumption.
+        -- intros Hcon.
+           apply H0.
+           apply AFI_LetNonRec.
+           assumption.
+        -- assumption.
+      * unfold P_Term in H.
+        apply H with x s.
+        -- intros Hcon.
+           apply H0.
+           apply AFI_Let.
+           assumption.
+        -- assumption.
+    + (* S_LetRec1 *)
+      reflexivity.
+    + (* S_LetRec2 *)
+      f_equal.
+      * assert (P_Bindings_Rec bs) by apply P_Bindings_Rec__holds_definitionally.
+        unfold P_Bindings_Rec in H2.
+        apply H2 with x s.
+        -- assumption.
+        -- intros Hcon.
+           apply H0.
+           apply AFI_LetRec.
+           ++ assumption.
+           ++ assumption.
+        -- assumption.
+      * unfold P_Term in H.
+        apply H with x s.
+        -- intros Hcon.
+           apply H0.
+           apply AFI_Let.
+           assumption.
+        -- assumption.
+  - (* Var *)
+    intros. unfold P_Term. intros.
+    inversion H0.
+    + (* S_Var1 *)
+      subst.
+      assert (appears_free_in s (Var s)) by constructor.
+      apply H in H1.
+      destruct H1.
+    + (* S_Var2 *)
+      reflexivity.
+  - (* TyAbs *)
+    intros. unfold P_Term. intros.
+    inversion H1. subst.
+    f_equal.
+    unfold P_Term in H.
+    apply H with x s0.
+    + intros Hcon.
+      apply H0.
+      apply AFI_TyAbs.
+      assumption.
+    + assumption.
+  - (* LamAbs *)
+    intros. unfold P_Term. intros.
+    inversion H1.
+    + (* S_LamAbs1 *)
+      reflexivity.
+    + (* S_LamAbs2 *)
+      subst.
+      f_equal.
+      unfold P_Term in H.
+      apply H with x s0.
+      * intros Hcon.
+        apply H0.
+        apply AFI_LamAbs.
+        assumption.
+      * assumption.
+  - (* Apply *)
+    intros. unfold P_Term. intros.
+    inversion H2. subst.
+    f_equal.
+    + unfold P_Term in H. 
+      apply H with x s.
+      * intros Hcon.
+        apply H1.
+        apply AFI_Apply1.
+        assumption.
+      * assumption.
+    + unfold P_Term in H0.
+      apply H0 with x s.
+      * intros Hcon.
+        apply H1.
+        apply AFI_Apply2.
+        assumption.
+      * assumption.
+  - (* Constant *)
+    intros. unfold P_Term. intros.
+    inversion H0. subst.
+    reflexivity.
+  - (* Builtin *)
+    intros. unfold P_Term. intros.
+    inversion H0. subst.
+    reflexivity.
+  - (* TyInst *)
+    intros. unfold P_Term. intros.
+    inversion H1. subst.
+    f_equal.
+    unfold P_Term in H.
+    apply H with x s.
+    + intros Hcon.
+      apply H0.
+      apply AFI_TyInst.
+      assumption.
+    + assumption.
+  - (* Error *)
+    intros. unfold P_Term. intros.
+    inversion H0. subst.
+    reflexivity.
+  - (* IWrap *)
+    intros. unfold P_Term. intros.
+    inversion H1. subst.
+    f_equal.
+    unfold P_Term in H.
+    apply H with x s.
+    + intros Hcon.
+      apply H0.
+      apply AFI_IWrap.
+      assumption.
+    + assumption.
+  - (* Unwrap *)
+    intros. unfold P_Term. intros.
+    inversion H1. subst.
+    f_equal.
+    unfold P_Term in H.
+    apply H with x s.
+    + intros Hcon.
+      apply H0.
+      apply AFI_Unwrap.
+      assumption.
+    + assumption.
+
+  - (* TermBind *)
+    intros. unfold P_Binding. intros.
+    inversion H1. subst.
+    f_equal.
+    unfold P_Term in H.
+    apply H with x s0.
+    + intros Hcon.
+      apply H0.
+      apply AFI_TermBind.
+      assumption.
+    + assumption.
+  - (* TypeBind *)
+    intros. unfold P_Binding. intros.
+    inversion H0. subst.
+    reflexivity.
+  - (* DatatypeBind *)
+    intros. unfold P_Binding. intros.
+    inversion H0. subst.
+    reflexivity.
+Qed.
+
+Lemma subst_closed : forall t,
+    closed t -> 
+    forall x s t',
+      substitute x s t t' ->
+      t' = t.
+Proof. Admitted.
+
+Lemma subst_not_afi : forall t x v,
+    closed v ->
+    forall t',
+      substitute x v t t' ->
+      ~(appears_free_in x t').
+Proof. Admitted.
+
+Lemma duplicate_subst : forall x t v s,
+    closed v ->
+    forall t' t'',
+      substitute x v t t' ->
+      substitute x s t' t'' ->
+      t'' = t'.
+Proof. Admitted.
+
+Lemma swap_subst : forall t x x1 v v1,
+    x <> x1 ->
+    closed v ->
+    closed v1 ->
+    forall t1 t2 t3 t4,
+      substitute x v t t1 ->
+      substitute x1 v1 t1 t2 ->
+      substitute x1 v1 t t3 ->
+      substitute x v t3 t4 ->
+      t2 = t4.
+Proof. Admitted.
+
+
+
+(** ** Properties of multi-substitutions *)
+
+Lemma msubst_closed : forall t,
+    closed t ->
+    forall ss t',
+      msubst ss t t' ->
+      t' = t.
+Proof. Admitted.
+
+Fixpoint closed_env (env : env) :=
+  match env with
+  | nil => True
+  | (x,t) :: env' => closed t /\ closed_env env'
+  end.
+
+Lemma subst_msubst : forall env x v t,
+    closed v ->
+    closed_env env ->
+    forall t1 t2 t3 t4,
+      substitute x v t t1 ->
+      msubst env t1 t2 ->
+      msubst (drop x env) t t3 ->
+      substitute x v t3 t4 ->
+      t2 = t4.
+Proof. Admitted.
+
+Lemma msubst_Var : forall ss x,
+    closed_env ss ->
+    forall t',
+      msubst ss (Var x) t' ->
+      t' =
+        match lookup x ss with
+        | Datatypes.Some t => t 
+        | None=> Var x
+        end.
+Proof. 
+  induction ss; intros.
+  - inversion H0. subst. 
+    reflexivity.
+  - inversion H0. subst.
+    simpl.
+    inversion H3; subst.
+    + rewrite String.eqb_refl.
+      eapply msubst_closed; eauto.
+      inversion H; auto.
+    + apply String.eqb_neq in H5.
+      rewrite H5.
+      apply IHss; eauto.
+      inversion H; auto.
+Qed.
+
+Lemma msubst_Apply : forall ss t1 t2 t',
+    msubst ss (Apply t1 t2) t' ->
+    exists t1' t2', msubst ss t1 t1' /\ msubst ss t2 t2' /\ t' = (Apply t1' t2').
+Proof.
+  induction ss; intros.
+  - inversion H. subst.
+    exists t1, t2.
+    eauto using msubst_nil, msubst_cons. 
+  - inversion H. subst.
+    rename t'0 into t''.
+    inversion H2. subst.
+    apply IHss in H5.
+    destruct H5 as [t1'' [t2'' [H9 [H10 H11]]]].
+    exists t1'', t2''.
+    split. {
+      apply msubst_cons with t1'.
+      + assumption.
+      + apply H9.
+    }
+    split. {
+      apply msubst_cons with t2'.
+      + assumption.
+      + apply H10.
+    }
+    assumption.
+Qed.
+
+(** ** Properties of multi-extensions *)
+
+Lemma mupdate_lookup : forall (c : tass) (x : name),
+    lookup x c = lookupT (mupdate emptyContext c) x.
+Proof. Admitted.
+
+Lemma mupdate_drop : forall (c : tass) Gamma x x',
+      lookupT (mupdate Gamma (drop x c)) x' 
+    = if String.eqb x x' 
+        then lookupT Gamma x' 
+        else lookupT (mupdate Gamma c) x'.
+Proof. Admitted.
+
+
+
+(** ** Properties of Instantiations *)
+
+Lemma instantiation_domains_match : forall c e1 e2,
+    instantiation c e1 e2 ->
+    forall x T,
+      lookup x c = Datatypes.Some T ->
+      exists t1 t2,
+        lookup x e1 = Datatypes.Some t1 /\
+        lookup x e2 = Datatypes.Some t2.
+Proof.
+  intros c e1 e2 V. 
+  induction V; intros x0 T0 C.
+  - discriminate.
+  - simpl.
+    simpl in C.
+    destruct (x =? x0) eqn:Heqb.
+    + eauto.
+    + apply IHV with T0.
+      assumption.
+Qed.
+
+Lemma instantiation_env_closed : forall c e1 e2,
+    instantiation c e1 e2 ->
+    closed_env e1 /\ closed_env e2.
+Proof.
+  intros c e1 e2 V.
+  induction V; intros.
+  - split; reflexivity.
+  - split.
+    + simpl.
+      split.
+      * apply typable_empty__closed with T.
+        apply R_typable_empty_1 with v2.
+        assumption.
+      * apply IHV.
+    + simpl.
+      split.
+      * apply typable_empty__closed with T.
+        apply R_typable_empty_2 with v1.
+        assumption.
+      * apply IHV.
+Qed.
+    
+
+Corollary instantiation_env_closed_1 : forall c e1 e2,
+    instantiation c e1 e2 ->
+    closed_env e1.
+Proof. intros. destruct (instantiation_env_closed _ _ _ H). assumption. Qed.
+
+Corollary instantiation_env_closed_2 : forall c e1 e2,
+    instantiation c e1 e2 ->
+    closed_env e2.
+Proof. intros. destruct (instantiation_env_closed _ _ _ H). assumption. Qed.
+
+Lemma instantiation_R : forall c e1 e2,
+    instantiation c e1 e2 ->
+    forall x T v1 v2,
+      lookup x c = Datatypes.Some T ->
+      lookup x e1 = Datatypes.Some v1 ->
+      lookup x e2 = Datatypes.Some v2 ->
+      R T v1 v2.
+Proof.
+  intros c e1 e2 V.
+  induction V; intros x' T' v1' v2' G E1 E2.
+  - destruct x'; discriminate.
+  - inversion G. subst.
+    inversion E1. subst.
+    inversion E2. subst.
+    destruct (x =? x').
+    + inversion H3. subst.
+      inversion H4. subst.
+      inversion H5. subst.
+      assumption. 
+    + apply IHV with x'; assumption.
+Qed.
+
+Lemma instantiation_drop : forall c e1 e2,
+    instantiation c e1 e2 ->
+    forall x,
+      instantiation (drop x c) (drop x e1) (drop x e2).
+Proof.
+  intros c e1 e2 V.
+  induction V.
+  - intros. simpl. apply V_nil.
+  - intros. simpl.
+    destruct (x =? x0).
+    + apply IHV.
+    + apply V_cons.
+      * assumption.
+      * assumption.
+      * assumption.
+      * apply IHV.
+Qed.
+
+(** ** Congruence lemmas on [eval] *)
+
+(** ** Multi-substitutions preserve typing *)
+
+Lemma msubst_preserves_typing_1 : forall c e1 e2,
+    instantiation c e1 e2 ->
+    forall Gamma t t' S,
+      (mupdate Gamma c) |-+ t : S ->
+      msubst e1 t t' ->
+      Gamma |-+ t': S. 
+Proof.
+  intros c e1 e2 V.
+  induction V.
+  - intros.
+    simpl in H.
+    inversion H0. subst.
+    assumption.
+  - intros.
+    simpl in H2.
+    inversion H3. subst.
+    apply IHV with t'0.
+    + eapply substitution_preserves_typing.
+      * apply H2.
+      * apply R_typable_empty_1 with v2.
+        apply H1.
+      * apply H9.
+    + apply H10.
+Qed. 
+
+Lemma msubst_preserves_typing_2 : forall c e1 e2,
+    instantiation c e1 e2 ->
+    forall Gamma t t' S,
+      (mupdate Gamma c) |-+ t : S ->
+      msubst e2 t t' ->
+      Gamma |-+ t': S. 
+Proof.
+  intros c e1 e2 V.
+  induction V.
+  - intros.
+    simpl in H.
+    inversion H0. subst.
+    assumption.
+  - intros.
+    simpl in H2.
+    inversion H3. subst.
+    apply IHV with t'0.
+    + eapply substitution_preserves_typing.
+      * apply H2.
+      * apply R_typable_empty_2 with v1.
+        apply H1.
+      * apply H9.
+    + apply H10.
+Qed. 
+
+(** ** The [R] Lemma *)
+
+Definition P_has_type ctx t1 T := 
+  forall c e1 e2 t2,
+    ctx = mupdate emptyContext c ->
+    ctx |-+ t1 : T ->
+    ctx |-+ t2 : T ->
+    instantiation c e1 e2 ->
+    CNR_Term t1 t2 ->
+    forall t1' t2',
+      msubst e1 t1 t1' ->
+      msubst e2 t2 t2' ->
+      R T t1' t2'.
+
+Definition P_constructor_well_formed ctx c := ctx |-ok_c c.
+
+Definition P_bindings_well_formed_nonrec ctx bs1 := ctx |-oks_nr bs1.
+
+Definition P_bindings_well_formed_rec ctx bs1 := ctx |-oks_r bs1.
+
+Definition P_binding_well_formed ctx b1 := ctx |-ok b1.
+
+Axiom skip : forall P, P.
+
+ (*forall c e1 e2 t1 t2 T,
+    (mupdate emptyContext c) |-+ t1 : T ->
+    (mupdate emptyContext c) |-+ t2 : T ->
+    instantiation c e1 e2 ->
+    CNR_Term t1 t2 ->
+    forall t1' t2',
+      msubst e1 t1 t1' ->
+      msubst e2 t2 t2' ->
+      R T t1' t2'.*)
+
+Lemma msubst_R : forall ctx t1 T,
+    ctx |-+ t1 : T ->
+    P_has_type ctx t1 T.
+Proof.
+  apply has_type__ind with 
+    (P := P_has_type)
+    (P0 := P_constructor_well_formed)
+    (P1 := P_bindings_well_formed_nonrec)
+    (P2 := P_bindings_well_formed_rec)
+    (P3 := P_binding_well_formed).
+  - intros. unfold P_has_type. intros. subst.
+    apply skip.
+  - intros. unfold P_has_type. intros. subst.
+    apply skip.
+
+  - (* T_Var *)
+    intros. 
+    unfold P_has_type. 
+    intros c e1 e2 t2 Heq Ht1 Ht2 V Hds t1' t2' X1 X2.
+    subst.
+
+    inversion Hds. subst.
+    inversion X. subst.
+
+    assert (forall x, lookupT (mupdate emptyContext c) x = lookup x c). {
+      intros. rewrite mupdate_lookup. auto.
+    }
+    rewrite H0 in H.
+    destruct (instantiation_domains_match _ _ _ V _ _ H) as [t1'' [t2'' [Ht1'' Ht2'']]].
+    destruct (instantiation_env_closed _ _ _ V) as [He1 He2].
+    apply instantiation_R with c e1 e2 x.
+    + assumption.
+    + assumption.
+    + rewrite msubst_Var with e1 x t1'.
+      * rewrite Ht1''.
+        reflexivity.
+      * assumption.
+      * assumption.
+    + rewrite msubst_Var with e2 x t2'.
+      * rewrite Ht2''.
+        reflexivity.
+      * assumption.
+      * assumption.
+
+  - (* T_Forall *)
+    apply skip.
+
+  - (* T_LamAbs *)
+    apply skip.
+
+  - (* T_Apply *)
+    intros ctx t1_1 t1_2 T1 T2 Ht1_1 IH1_1 Ht1_2 IH1_2.
+    unfold P_has_type.
+    intros c e1 e2 t2 Heq Ht1 Ht2 V Hds t1' t2' Hms1 Hms2.
+    subst.
+
+    inversion Hds. subst.
+    inversion X. subst.
+    rename s' into t2_1.
+    rename t' into t2_2.
+    destruct (msubst_Apply _ _ _ _ Hms1) as [t1_1' [t1_2' [Hms_t1_1' [Hms_t1_2' Heq1']]]].
+    destruct (msubst_Apply _ _ _ _ Hms2) as [t2_1' [t2_2' [Hms_t2_1' [Hms_t2_2' Heq2']]]].
+    subst.
+
+    assert (emptyContext |-+ (Apply t1_1' t1_2') : T2) by eauto using msubst_preserves_typing_1.
+    assert (emptyContext |-+ (Apply t2_1' t2_2') : T2) by eauto using msubst_preserves_typing_2.
+
+    destruct (progress _ _ H) as [v1 Hv1].
+    destruct (progress _ _ H0) as [v2 Hv2].
+
+    assert (R (Ty_Fun T1 T2) t1_1' t2_1'). {
+      unfold P_has_type in IH1_1.
+      apply IH1_1 with c e1 e2 t2_1.
+      - reflexivity.
+      - assumption.
+      - eapply CNR_Term__preserves_typing; eauto.
+      - apply V.
+      - assumption.
+      - assumption.
+      - assumption.
+    }
+
+    assert (R T1 t1_2' t2_2'). {
+      unfold P_has_type in IH1_2.
+      apply IH1_2 with c e1 e2 t2_2. 
+      - reflexivity.
+      - assumption.
+      - eapply CNR_Term__preserves_typing; eauto.
+      - apply V.
+      - assumption.
+      - assumption.
+      - assumption.
+    }
+
+    destruct T2.
+    + (* Ty_Var *) 
+      apply R_functional_extensionality in H1.
+      destruct H1 as [v1' [v2' [Hv1' [Hv2' Hfe]]]].
+      apply Hfe in H2.
+      apply R_falsity in H2.
+      destruct H2.
+    + (* Ty_Fun *)
+      split; auto.
+      split; auto.
+      exists v1.
+      exists v2.
+      split; auto.
+      split; auto.
+
+      destruct (R_functional_extensionality _ _ _ _ H1) as [v1_1' [v2_1' [Hv1_1' [Hv2_1' Hfe']]]].
+      apply Hfe' in H2.
+
+      destruct (R_functional_extensionality _ _ _ _ H2) as [v1' [v2' [Hv1' [Hv2' Hfe]]]].
+
+      assert (Apply v1_1' t1_2' ==> v1). {
+        eapply eval_congr_Apply1.
+        - apply Hv1.
+        - assumption.
+      }
+      assert (Apply v2_1' t2_2' ==> v2). {
+        eapply eval_congr_Apply1.
+        - apply Hv2.
+        - assumption.
+      }
+
+      assert (v1 = v1') by (eapply eval__deterministic; eauto).
+      assert (v2 = v2') by (eapply eval__deterministic; eauto).
+      subst.
+      apply Hfe.
+    + (* Ty_IFix *)
+      split; auto.
+      split; auto.
+      eexists.
+      eexists.
+      eauto.
+    + (* Ty_Forall *)
+      split; auto.
+      split; auto.
+      eexists.
+      eexists.
+      eauto.
+    + (* Ty_Builtin *)
+      split; auto.
+      split; auto.
+      exists v1.
+      exists v2.
+      split; auto.
+      split; auto.
+
+      destruct (R_functional_extensionality _ _ _ _ H1) as [v1_1' [v2_1' [Hv1_1' [Hv2_1' Hfe']]]].
+      apply Hfe' in H2.
+
+      destruct (R_syntactic_equality _ _ _ H2) as [v1' [v2' [Hv1' [Hv2' Heq]]]].
+      subst.
+
+      assert (Apply v1_1' t1_2' ==> v1). {
+        eapply eval_congr_Apply1.
+        - apply Hv1.
+        - assumption.
+      }
+      assert (Apply v2_1' t2_2' ==> v2). {
+        eapply eval_congr_Apply1.
+        - apply Hv2.
+        - assumption.
+      }
+
+      assert (v1 = v2') by (eapply eval__deterministic; eauto).
+      assert (v2 = v2') by (eapply eval__deterministic; eauto).
+
+      subst.
+
+      reflexivity.
+
+    + (* Ty_Lam *)
+      apply R_functional_extensionality in H1.
+      destruct H1 as [v1' [v2' [Hv1' [Hv2' Hfe]]]].
+      apply Hfe in H2.
+      apply R_falsity in H2.
+      destruct H2.
+    + (* Ty_App *) 
+      apply R_functional_extensionality in H1.
+      destruct H1 as [v1' [v2' [Hv1' [Hv2' Hfe]]]].
+      apply Hfe in H2.
+      apply R_falsity in H2.
+      destruct H2.
+
+  - 
+
+Proof. Abort.
